1. clean up the specification of linkable extensions a bit 2. define the diagram property that handled calls must satisfy (each handled call is justified by a possibly extended, separated injection, etc., plus the usual conditions on match_states).  It remains to be seen how difficult it will be to prove this property for the concurrency extension, but it seems at least possible.  For extensions without multiple cores, I'm somewhat more confident.

veric/extensions.v
@@ -621,7 +621,7 @@ Qed.
 
 End SafetyCriteria.
 
-Section CorestepProperties.
+Section CoreCompat.
 Variables (G xT cT M D Z Zint Zext: Type) 
   (esem: CoreSemantics G xT M D) 
   (csem: nat -> option (CoreSemantics G cT M D))
@@ -632,37 +632,67 @@ Variables (G xT cT M D Z Zint Zext: Type)
 
 Import Extension.
 
-Definition runnable_corestep := forall ge s m s' m' c CS i,
-  runnable E ge s = Some i -> 
-  csem i = Some CS -> proj_core E s i = Some c -> 
-  corestep esem ge s m s' m' -> 
-  exists c', corestep CS ge c m c' m' /\ proj_core E s' i = Some c'.
+Inductive core_compat: Type := CoreCompat: forall
+  (runnable_corestep: forall ge s m s' m' c CS i,
+    runnable E ge s = Some i -> 
+    csem i = Some CS -> proj_core E s i = Some c -> 
+    corestep esem ge s m s' m' -> 
+    exists c', corestep CS ge c m c' m' /\ proj_core E s' i = Some c') 
+  (corestep_pres: forall ge c s m c' s' m' CS,
+    csem (active E s) = Some CS -> 
+    proj_core E s (active E s) = Some c -> 
+    corestep CS ge c m c' m' -> 
+    corestep esem ge s m s' m' -> 
+    (active E s = active E s' /\ runnable E ge s = runnable E ge s' /\ 
+      proj_core E s' (active E s) = Some c'))
+  (corestep_prog: forall ge c s m c' m' CS,
+    csem (active E s) = Some CS -> 
+    proj_core E s (active E s) = Some c -> 
+    corestep CS ge c m c' m' -> 
+    exists s', corestep esem ge s m s' m')
+  (corestep_others: forall ge i s c m s' c' m' CS,
+    csem i = Some CS -> proj_core E s' i = Some c' -> 
+    corestep CS ge c m c' m' -> 
+    corestep esem ge s m s' m' -> 
+    forall j, i<>j -> proj_core E s j = proj_core E s' j) 
+  (safely_halted_steps: forall ge s c rv m (CS: CoreSemantics G cT M D),
+    proj_core E s (active E s) = Some c -> 
+    safely_halted CS ge c = Some rv -> 
+    exists s', corestep esem ge s m s' m), 
+  core_compat.
 
-Definition corestep_active := forall ge c s m c' s' m' CS,
+Variable Hcore_compat: core_compat.
+
+Lemma corestep_step: forall ge c s m c' m' CS,
   csem (active E s) = Some CS -> 
   proj_core E s (active E s) = Some c -> 
   corestep CS ge c m c' m' -> 
-  corestep esem ge s m s' m' -> 
-  (active E s = active E s' /\ proj_core E s' (active E s) = Some c').
-
-Definition corestep_step := forall ge c s m c' m' CS,
-  csem (active E s) = Some CS -> 
-  proj_core E s (active E s) = Some c -> 
-  corestep CS ge c m c' m' -> 
-  exists s', corestep esem ge s m s' m' /\ (*conditions somewhat redundant*) 
-    active E s = active E s' /\
+  exists s', corestep esem ge s m s' m' /\
+    active E s = active E s' /\ runnable E ge s = runnable E ge s' /\
     proj_core E s' (active E s) = Some c'.
+Proof.
+intros.
+inv Hcore_compat.
+generalize H1 as H1'; intro.
+eapply corestep_prog in H1; eauto.
+destruct H1 as [s' H1].
+exists s'.
+split; auto. 
+eapply corestep_pres; eauto.
+Qed.
 
-Lemma corestep_step_plus: corestep_step -> 
+Lemma corestep_step_plus: 
   forall ge c s m c' m' CS,
   csem (active E s) = Some CS -> 
   proj_core E s (active E s) = Some c -> 
   corestep_plus CS ge c m c' m' -> 
   exists s', corestep_plus esem ge s m s' m' /\ 
-    active E s = active E s' /\
+    active E s = active E s' /\ runnable E ge s = runnable E ge s' /\
     proj_core E s' (active E s) = Some c'.
 Proof.
-intros H1; intros until CS; intros H2 H3 H4.
+inv Hcore_compat.
+generalize corestep_step; intro H1.
+intros until CS; intros H2 H3 H4.
 inversion H4 as [n H5]; clear H4; revert c c' m m' s H2 H3 H5; induction n. 
 intros c c' m m' s H2 H3 H5.
 inv H5.
@@ -678,29 +708,32 @@ intros c c' m m' s H2 H3 H5.
 simpl in H5.
 destruct H5 as [c2 [m2 [H5 H6]]].
 eapply H1 in H5; eauto.
-destruct H5 as [s2 [H5 [H7 H8]]].
-rewrite H7 in H2, H8.
-destruct (IHn c2 c' m2 m' s2 H2 H8) as [s' [H9 [H10 H11]]]; auto.
+destruct H5 as [s2 [H5 [H7 [H8 H9]]]].
+rewrite H7 in H2. 
+destruct (IHn c2 c' m2 m' s2 H2) as [s' [H10 [H11 [H12 H13]]]]; auto.
+rewrite <-H7; auto.
 exists s'.
 split3.
-inv H9.
+inv H10.
 exists (S x).
 simpl.
 exists s2; exists m2; split; auto.
 rewrite H7; auto.
-rewrite H7, H11; auto.
+rewrite H8, H12.
+rewrite H7; split; auto.
 Qed.
 
-Lemma corestep_step_star: corestep_step -> 
+Lemma corestep_step_star:
   forall ge c s m c' m' CS,
   csem (active E s) = Some CS -> 
   proj_core E s (active E s) = Some c -> 
   corestep_star CS ge c m c' m' -> 
   exists s', corestep_star esem ge s m s' m' /\ 
-    active E s = active E s' /\
+    active E s = active E s' /\ runnable E ge s = runnable E ge s' /\
     proj_core E s' (active E s) = Some c'.
 Proof.
-intros H1; intros until CS; intros H2 H3 H4.
+generalize corestep_step; intro H1.
+intros until CS; intros H2 H3 H4.
 inversion H4 as [n H5]; clear H4; revert c c' m m' s H2 H3 H5; induction n. 
 intros c c' m m' s H2 H3 H5.
 inv H5.
@@ -710,31 +743,22 @@ intros c c' m m' s H2 H3 H5.
 simpl in H5.
 destruct H5 as [c2 [m2 [H5 H6]]].
 eapply H1 in H5; eauto.
-destruct H5 as [s2 [H5 [H7 H8]]].
-rewrite H7 in H2, H8.
-destruct (IHn c2 c' m2 m' s2 H2 H8) as [s' [H9 [H10 H11]]]; auto.
+destruct H5 as [s2 [H5 [H7 [H8 H9]]]].
+rewrite H7 in H2. 
+destruct (IHn c2 c' m2 m' s2 H2) as [s' [H10 [H11 [H12 H13]]]]; auto.
+rewrite <-H7; auto.
 exists s'.
 split3.
-inv H9.
+inv H10.
 exists (S x).
 simpl.
 exists s2; exists m2; split; auto.
 rewrite H7; auto.
-rewrite H7, H11; auto.
+rewrite H8, H12.
+rewrite H7; split; auto.
 Qed.
 
-Definition corestep_others := forall ge i s c m s' c' m' (CS: CoreSemantics G cT M D),
-  proj_core E s' i = Some c' -> 
-  corestep CS ge c m c' m' -> 
-  corestep esem ge s m s' m' -> 
-  forall j, i<>j -> proj_core E s j = proj_core E s' j.
-
-Definition safely_halted_steps := forall ge s c rv m (CS: CoreSemantics G cT M D),
-  proj_core E s (active E s) = Some c -> 
-  safely_halted CS ge c = Some rv -> 
-  exists s', corestep esem ge s m s' m.
-
-End CorestepProperties.
+End CoreCompat.
     
 Section LinkableExtension.
 Variables (fT: forall X:Type, Type) (cT dT D Z Zint Zext: Type)
@@ -783,16 +807,8 @@ Definition match_states (cd: core_data core_simulation) (j: meminj) (s1: xT) m1 
       match_state core_simulation cd j c1 m1 c2 m2.
 
 Inductive linkable_extension: Type := LinkableExtension: forall 
-  (runnable_corestep1: runnable_corestep E1)
-(*  (runnable_corestep2: runnable_corestep E2)*)
-  (corestep_active1: corestep_active E1)
-(*  (corestep_active2: corestep_active E2)*)
-(*  (corestep_step1: corestep_step E1)*)
-  (corestep_step2: corestep_step E2)
-  (corestep_others1: corestep_others E1)
-(*  (corestep_others2: corestep_others E2)*)
-(*  (safely_halted_steps1: safely_halted_steps E1)
-  (safely_halted_steps2: safely_halted_steps E2)*)
+  (core_compat1: core_compat E1)
+  (core_compat2: core_compat E2)
   (match_mem_inject: forall cd j c1 c2 m1 m2,
     match_state core_simulation cd j c1 m1 c2 m2 -> 
     Mem.inject j m1 m2)
@@ -812,7 +828,25 @@ Inductive linkable_extension: Type := LinkableExtension: forall
       inject_incr j j' /\
       Events.inject_separated j j' m1 m2 /\
       corestep (esem target) ge s2 m2 s2' m2' /\
-      match_states cd' j' s1' m1' s2' m2'), 
+      match_states cd' j' s1' m1' s2' m2')
+  (extension_diagram: forall c1 s1 m1 s1' m1' c2 s2 m2 ef sig args1 args2 cd j,
+    ACTIVE E1 s1 = ACTIVE E2 s2 -> 
+    RUNNABLE E1 ge s1 = None -> RUNNABLE E2 ge s2 = None -> 
+    PROJ_CORE E1 s1 (ACTIVE E1 s1) = Some c1 -> 
+    PROJ_CORE E2 s2 (ACTIVE E2 s2) = Some c2 -> 
+    at_external source c1 = Some (ef, sig, args1) -> 
+    at_external target c2 = Some (ef, sig, args2) -> 
+    match_states cd j s1 m1 s2 m2 -> 
+    Mem.inject j m1 m2 -> 
+    Events.meminj_preserves_globals ge j -> 
+    Forall2 (val_inject j) args1 args2 -> 
+    Forall2 Val.has_type args2 (sig_args sig) -> 
+    corestep (esem source) ge s1 m1 s1' m1' -> 
+    exists s2', exists m2', exists cd', exists j',
+      inject_incr j j' /\
+      Events.inject_separated j j' m1 m2 /\
+      match_states cd' j' s1' m1' s2' m2' /\
+      corestep (esem target) ge s2 m2 s2' m2'),
   linkable_extension.
 
 Variable (esig_linkable: linkable_extension).
@@ -837,9 +871,9 @@ destruct (active_proj_core E1 st1) as [c1 H2].
 rewrite H1 in H2.
 assert (exists c1', corestep source ge c1 m1 c1' m1').
  inv esig_linkable.
- unfold runnable_corestep in runnable_corestep1.
- specialize (runnable_corestep1 ge st1 m1 st1' m1' c1 source (ACTIVE E1 st1)).
- destruct runnable_corestep1 as [c1' [H3 H4]]; auto.
+ inv core_compat1.
+ specialize (runnable_corestep ge st1 m1 st1' m1' c1 source (ACTIVE E1 st1)).
+ destruct runnable_corestep as [c1' [H3 H4]]; auto.
  exists c1'; auto.
 destruct H3 as [c1' H3].
 generalize (core_diagram core_simulation).
@@ -865,16 +899,28 @@ rewrite <-X0 in H10.
 inv esig_linkable; eauto.
 rewrite <-H10.
 inv esig_linkable.
-eapply corestep_active1 in H3; eauto.
+inv core_compat1.
+eapply corestep_pres in H3; eauto.
 destruct H3; eauto.
 rewrite <-H1; auto.
 split.
-admit. (*RUNNABLE*)
+destruct H11; auto.
+rewrite <-H11.
+rewrite <-X1.
+inv esig_linkable.
+inv core_compat1.
+eapply corestep_pres in H.
+destruct H as [? [? ?]]; auto.
+unfold cores; simpl; eauto.
+eauto.
+eapply H3.
 intros i c0 H12.
 assert (H13: PROJ_CORE E1 st1' n = Some c1'). 
  inv esig_linkable.
- edestruct corestep_active1; eauto.
+ inv core_compat1.
+ edestruct corestep_pres; eauto.
  unfold cores; auto.
+ destruct H13; auto.
 case_eq (eq_nat_dec i n).
 (*i=n*)
 intros Heq _.
@@ -883,11 +929,14 @@ rewrite H13 in H12.
 inv H12.
 exists c2'.
 rewrite X0; split; auto.
+destruct H11; auto.
 (*i<>n*)
 intros Hneq _.
 assert (PROJ_CORE E1 st1 i = Some c0). 
  inv esig_linkable.
- erewrite corestep_others1; eauto.
+ inv core_compat1.
+ erewrite corestep_others; eauto.
+ unfold cores; auto.
 unfold match_states in H0'.
 destruct (H0'' i c0 H14) as [c3 [H15 H16]].
 exists c3.
@@ -935,9 +984,17 @@ unfold match_states in H0.
 destruct (H0 (ACTIVE E1 st1) c1 H1) as [c2 [H4 H5]].
 destruct (core_at_external core_simulation cd j c1 m1 c2 m2 ef args sig H5 H2)
  as [H6 [H7 [vals2 [H8 [H9 H10]]]]].
-admit. (*here we need the user to prove a "core diagram" for external function 
-          calls handled by the extension; there must be an appropriate (extended)
-          injection to justify each step that handles one of these calls*)
+inv esig_linkable. 
+edestruct extension_diagram as [s2' H11]; eauto.
+rewrite <-X1; auto.
+rewrite <-X0; auto.
+destruct H11 as [m2' [cd' [j' [? [? [? ?]]]]]].
+exists s2'; exists m2'; exists cd'; exists j'.
+split3; auto.
+split; auto.
+left. 
+exists 0%nat; simpl. 
+eexists; eexists; split; eauto.
 Qed.
 Next Obligation. Admitted. (*TODO*)
 Next Obligation. Admitted. (*TODO*)
